verif/btrees/abstract_spec.v
@@ -1,6 +1,118 @@
 (*  *)
 Require Import index.
 Require Import btrees.
+Require Import btrees_sep.
 Require Import Int.
 Require Import BTrees.
 Require Import BTreesModule.
+Require Import Omega.
+Require Import Coq.Lists.List.
+Require Import FunInd.
+Require Import Int.
+Require Import VST.floyd.proofauto.
+Require Import VST.floyd.library.
+
+Module BTree <: CURSOR_TABLE.
+ Definition key := btrees.key.
+
+ Definition lt_key := Int.lt. 
+  
+ Definition V := btrees.V.
+
+ Definition table := btrees.relation unit. (* unit? X? *)
+ Definition cursor := prod (btrees.cursor unit) (btrees.relation unit).
+ Definition empty_t : table := btrees.empty_relation tt tt.
+
+ Definition make_cursor (k: key) (m: table) : cursor :=
+   (btrees.moveToKey unit (btrees.get_root m) k [], m).
+ 
+ Definition get_table (c : cursor) : table := snd c.
+ 
+ Definition get_key (c: cursor) : option key :=
+   GetKey (fst c) (snd c).
+   
+ Definition get (c: cursor) : option V :=
+   GetRecord (fst c) (snd c).
+   
+ Definition insert (c: cursor) (k: key) (v: V) : cursor :=
+   RL_PutRecord (fst c) (snd c) k v tt [] tt.
+   
+ Definition next (c: cursor) : cursor :=
+   (moveToNext (fst c) (snd c), snd c).
+   
+ Definition prev (c: cursor) : cursor :=
+   (moveToPrev (fst c) (snd c), snd c).
+   
+ Definition first_cursor (m: table) : cursor :=
+   (btrees.first_cursor (btrees.get_root m),m).
+   
+ Definition last_cursor (m: table) : cursor :=
+   (btrees.last_cursor (btrees.get_root m),m).
+ 
+ Definition abs_rel (m: table) (c: cursor) : Prop :=
+   m = snd c.
+   
+ Definition key_rel (k: key) (c: cursor) : Prop := True. (* TODO *)
+ 
+ Definition eq_cursor c1 c2 : Prop :=
+   btrees.normalize (fst c1) (snd c2) = btrees.normalize (X:=unit) (fst c2) (snd c2) /\ snd c1 = snd c2.
+   
+ Definition cursor_correct (c: cursor) : Prop :=
+   complete_cursor (fst c) (snd c).
+ 
+ Definition table_correct (t: table) : Prop :=
+   True.
+
+ (* table-cursor relations *)
+ Theorem make_cursor_rel: forall t k,
+   abs_rel t (make_cursor k t).
+ Proof. Admitted.
+ Theorem get_table_rel: forall t c,
+   abs_rel t c <-> get_table c = t.
+ Proof. Admitted.
+ Theorem first_rel: forall t,
+   abs_rel t (first_cursor t).
+ Proof. Admitted.
+ Theorem last_rel: forall t,
+   abs_rel t (last_cursor t).
+ Proof. Admitted.
+ Theorem next_rel: forall t c,
+   abs_rel t c -> abs_rel t (next c).
+ Proof. Admitted.
+ Theorem prev_rel: forall t c,
+   abs_rel t c -> abs_rel t (prev c).
+ Proof. Admitted.
+ Theorem correct_rel: forall t c,
+   abs_rel t c -> (cursor_correct c <-> table_correct t).
+ Proof. Admitted.
+
+ (* correctness preservation *)
+ Theorem insert_correct: forall k v c,
+   cursor_correct c -> key_rel k c -> cursor_correct (insert c k v).
+ Proof. Admitted.
+
+ (* get/insert correctness *)
+ Theorem glast: forall t,
+   get (last_cursor t) = None.
+ Proof. Admitted.
+ Theorem gis: forall k v c,
+   cursor_correct c -> key_rel k c ->
+   get (make_cursor k (get_table (insert c k v))) = Some v.
+ Proof. Admitted.
+ Theorem gio: forall j k v c,
+   cursor_correct c -> key_rel k c -> ~ key_rel j c ->
+   get (make_cursor j (get_table (insert c k v))) =
+   get (make_cursor j (get_table c)).
+ Proof. Admitted.
+
+ (* cursor movement *)
+ Theorem next_prev: forall c t,
+   cursor_correct c -> abs_rel t c -> ~ (c = last_cursor t) -> eq_cursor c (prev (next c)).
+ Proof. Admitted.
+ Theorem prev_next: forall c t,
+   cursor_correct c -> abs_rel t c -> ~ (c = first_cursor t) -> eq_cursor c (next (prev c)).
+ Proof. Admitted.
+ Theorem cursor_order: forall c k1 k2,
+   cursor_correct c -> get_key c = Some k1 -> get_key (next c) = Some k2 -> lt_key k1 k2 = true.
+ Proof. Admitted.
+End BTree.
